LoL/MonadUtil.lean
@@ -1,4 +1,5 @@
 import Mathlib.Order.Basic
+import Mathlib.Order.Lattice
 
 universe u v w
 
@@ -40,6 +41,9 @@ instance (t : Type v) [Preorder t] : Monad (W t) where
   pure x := ⟨fun f => f x, by solve_by_elim⟩
   bind x f := ⟨fun g => x.wp (fun a => (f a).wp g), by simp; intros; solve_by_elim [W.wp_montone]⟩
 
-class Logic (t : Type u) extends PartialOrder t where
-  and : t -> t -> t
-  pure : Prop -> t
+-- class Logic (t : Type u) extends SemilatticeInf t where
+--   pure : Prop -> t
+--   and_pure : ∀ p₁ p₂, pure p₁ ⊓ pure p₁ = pure (p₁ ∧ p₂)
+--   le_pure :  ∀ p₁ p₂, (p₁ -> p₂) -> pure p₁ ≤ pure p₂
+
+-- notation "⌜" p "⌝" => Logic.pure p
